code/ecdsa/Hacl.Impl.P256.Signature.Common.fsti
@@ -4,7 +4,6 @@ open FStar.HyperStack.All
 open FStar.HyperStack
 
 open Lib.IntTypes
-open Lib.ByteBuffer
 open Lib.ByteSequence
 open Lib.Buffer
 
@@ -13,80 +12,55 @@ open Spec.ECC.Curves
 open Hacl.Spec.EC.Definition
 
 open Spec.ECDSA
-(* open Spec.ECC.Lemmas *)
-open Hacl.Spec.ECDSA.Definition
-
-open Hacl.Impl.EC.Core
-
 open FStar.Mul
 
-#set-options "--fuel 0 --ifuel 0 --z3rlimit 200"
+#set-options "--fuel 0 --ifuel 0 --z3rlimit 100"
 
 val bufferToJac: #c: curve -> p: lbuffer uint64 (getCoordinateLenU64 c *. 2ul) -> result: point c -> Stack unit
   (requires fun h -> live h p /\ live h result /\ disjoint p result)
-  (ensures  fun h0 _ h1 ->
+  (ensures  fun h0 _ h1 -> modifies (loc result) h0 h1 /\ (
     let len = getCoordinateLenU64 c in 
-    modifies (loc result) h0 h1 /\
-    as_nat c h1 (gsub result (len *. size 2) len) == 1 /\
-    (
-      let x = as_nat c h0 (gsub p (size 0) len) in
-      let y = as_nat c h0 (gsub p len len) in
-      let x3, y3, z3 = point_x_as_nat c h1 result, point_y_as_nat c h1 result, point_z_as_nat c h1 result in
-      let pointJacX, pointJacY, pointJacZ = toJacobianCoordinates (x, y) in
-      x3 == pointJacX /\ y3 == pointJacY /\ z3 == pointJacZ)
-      )
-
+    let x, y = as_nat c h0 (gsub p (size 0) len),  as_nat c h0 (gsub p len len) in
+    point_eval c h1 result /\ (
+    let x3, y3, z3 = point_as_nat c h1 result in
+    let pointJacX, pointJacY, pointJacZ = toJacobianCoordinates (x, y) in 
+    as_nat c h1 (gsub result (len *. size 2) len) == 1 /\ x3 == pointJacX /\ y3 == pointJacY /\ z3 == pointJacZ)))
 
 
 [@ (Comment "  This code is not side channel resistant")]  
-val isPointAtInfinityPublic: #c: curve -> p:point c -> Stack bool
+val isPointAtInfinityPublic: #c: curve -> p: point c -> Stack bool
   (requires fun h -> live h p)
-  (ensures  fun h0 r h1 -> modifies0 h0 h1 /\
-    r == Spec.ECC.isPointAtInfinity (point_prime_to_coordinates c (as_seq h0 p)))
+  (ensures  fun h0 r h1 -> modifies0 h0 h1 /\ r == Spec.ECC.isPointAtInfinity (point_prime_to_coordinates c (as_seq h0 p)))
 
 
 [@ (Comment "  This code is not side channel resistant")]
 val isPointOnCurvePublic: #c: curve -> p: point c -> Stack bool
   (requires fun h -> 
     let len = getCoordinateLenU64 c in 
-    let prime = getPrime c in 
-    live h p /\    
-    as_nat c h (gsub p (size 0) len) < prime /\ 
-    as_nat c h (gsub p len len) < prime /\
+    live h p /\ felem_eval c h (gsub p (size 0) len) /\ felem_eval c h (gsub p len len) /\
     as_nat c h (gsub p (size 2 *! len) len) == 1)
   (ensures fun h0 r h1 ->
     let len = getCoordinateLenU64 c in 
     modifies0 h0 h1 /\ 
-    r == isPointOnCurve #c (as_nat c h1 (gsub p (size 0) len), 
-                          as_nat c h1 (gsub p len len), 
-                          as_nat c h1 (gsub p (size 2 *! len) len))
-  )
+    r == isPointOnCurve #c (as_nat c h1 (gsub p (size 0) len), as_nat c h1 (gsub p len len), as_nat c h1 (gsub p (size 2 *! len) len)))
 
 
 [@ (Comment "  This code is not side channel resistant")] 
-val verifyQValidCurvePoint: #c: curve -> pubKeyAsPoint: point c
-  -> tempBuffer:lbuffer uint64 (size 25 *! getCoordinateLenU64 c) -> Stack bool
-  (requires fun h ->
-    live h pubKeyAsPoint /\
-    live h tempBuffer /\
-    LowStar.Monotonic.Buffer.all_disjoint [loc pubKeyAsPoint; loc tempBuffer] /\
-    point_z_as_nat c h pubKeyAsPoint == 1
-  )
-  (ensures  fun h0 r h1 ->
-    modifies (loc tempBuffer) h0 h1 /\
+val verifyQValidCurvePoint: #c: curve -> pubKeyAsPoint: point c 
+  -> tempBuffer:lbuffer uint64 (size 25 *! getCoordinateLenU64 c) -> 
+  Stack bool
+  (requires fun h -> live h pubKeyAsPoint /\ live h tempBuffer /\
+    LowStar.Monotonic.Buffer.all_disjoint [loc pubKeyAsPoint; loc tempBuffer] /\ (
+    let len = getCoordinateLenU64 c in as_nat c h (gsub pubKeyAsPoint (size 2 *! len) len) == 1))
+  (ensures  fun h0 r h1 -> modifies (loc tempBuffer) h0 h1 /\
+    ~ (isPointAtInfinity ((point_prime_to_coordinates c (as_seq h0 pubKeyAsPoint)))) /\
     r == verifyQValidCurvePointSpec #c (point_prime_to_coordinates c (as_seq h0 pubKeyAsPoint)))
 
 
-val verifyQ: 
-  #c: curve ->
-  pubKey: lbuffer uint8 (size (getPointLen c)) ->
-  Stack bool
-    (requires fun h -> live h pubKey)
-    (ensures  fun h0 r h1 -> modifies0 h0 h1 /\
-      (
-	let publicKeyX = nat_from_bytes_be (as_seq h1 (gsub pubKey (size 0) (size (getCoordinateLen c)))) in 
-	let publicKeyY = nat_from_bytes_be (as_seq h1 (gsub pubKey (size (getCoordinateLen c)) (size (getCoordinateLen c)))) in
-	let pkJ = Spec.ECC.toJacobianCoordinates (publicKeyX, publicKeyY) in 
-	r == verifyQValidCurvePointSpec #c pkJ
-      )
-    )
+val verifyQ: #c: curve -> pubKey: lbuffer uint8 (size (getPointLen c)) -> Stack bool
+  (requires fun h -> live h pubKey)
+  (ensures  fun h0 r h1 -> modifies0 h0 h1 /\ (
+    let publicKeyX = nat_from_bytes_be (as_seq h1 (gsub pubKey (size 0) (size (getCoordinateLen c)))) in 
+    let publicKeyY = nat_from_bytes_be (as_seq h1 (gsub pubKey (size (getCoordinateLen c)) (size (getCoordinateLen c)))) in
+    let pkJ = Spec.ECC.toJacobianCoordinates (publicKeyX, publicKeyY) in 
+    r == verifyQValidCurvePointSpec #c pkJ))
