code/ecdsa/Hacl.Impl.ECDSA.LowLevel.fst
@@ -1,0 +1,105 @@
+module Hacl.Impl.ECDSA.LowLevel
+
+open FStar.HyperStack.All
+open FStar.HyperStack
+module ST = FStar.HyperStack.ST
+
+open Lib.IntTypes
+open Lib.Buffer
+
+open FStar.Math.Lemmas
+open Hacl.Impl.EC.LowLevel 
+
+open Hacl.Impl.EC.Masking
+open FStar.Mul
+open Lib.IntTypes.Intrinsics
+
+
+#reset-options "--z3rlimit 300"
+
+val lemma_reduction_prime_2prime_with_carry_cin: 
+  c: curve ->
+  cin: nat {cin <= 1} ->
+  x: nat {x + cin * pow2 (getPower c) < 2 * getOrder #c /\ x < pow2 (getPower c)} -> 
+  carry0 : nat {carry0 <= 1 /\ (if carry0 = 0 then x >= getOrder #c else x < getOrder #c)} -> 
+  result: nat {if cin < carry0 then result = x else result = x - getOrder #c + carry0 * pow2 (getPower c)} -> 
+  Lemma (result = (x + cin * pow2 (getPower c)) % getOrder #c)
+
+let lemma_reduction_prime_2prime_with_carry_cin c cin x carry0 result = 
+  let n = x + cin * pow2 (getPower c) in 
+  let prime = getOrder #c in 
+
+  if cin = 0 && carry0 = 1 then begin
+    small_mod x prime;
+    assert(result = (x + cin * pow2 (getPower c)) % prime)
+    end
+  else if cin = 0 && carry0 = 0 then begin
+    small_modulo_lemma_1 (x - prime) prime;
+    lemma_mod_sub x prime 1;
+    assert(result = (x + cin * pow2 (getPower c)) % prime)
+    end
+  else if cin = 1 && carry0 = 0 then 
+    assert(result = (x + cin * pow2 (getPower c)) % prime)
+  else
+    begin 
+      lemma_mod_sub (x + cin * pow2 (getPower c)) prime 1;
+      small_mod result prime;
+      assert(result = (x + cin * pow2 (getPower c)) % prime)
+    end
+
+
+val reduction_prime_2prime_with_carry_cin: #c: curve -> cin: uint64 -> x: felem c -> result: felem c ->
+  Stack unit
+  (requires fun h -> live h x /\ live h result /\ eq_or_disjoint x result /\ (
+    as_nat c h x + uint_v cin * pow2 (getPower c) < 2 * getOrder #c))
+  (ensures fun h0 _ h1 -> modifies (loc result) h0 h1 /\
+    as_nat c h1 result = (as_nat c h0 x + uint_v cin * pow2 (getPower c)) % getOrder #c)
+
+let reduction_prime_2prime_with_carry_cin #c cin x result =
+  push_frame();
+
+  let h0 = ST.get() in 
+
+  let len = getCoordinateLenU64 c in
+
+  let tempBuffer = create len (u64 0) in
+  let tempBufferForSubborrow = create (size 1) (u64 0) in
+ 
+  let carry0 = sub_bn_order x tempBuffer in
+  let carry = sub_borrow_u64 carry0 cin (u64 0) tempBufferForSubborrow in
+  cmovznz4 carry tempBuffer x result;
+  pop_frame();
+  
+  let h2 = ST.get() in 
+  lseq_upperbound #(v (getCoordinateLenU64 c)) (as_seq h0 x); 
+  lemma_reduction_prime_2prime_with_carry_cin c (v cin) (as_nat c h0 x) (uint_v carry0) (as_nat c h2 result)
+
+
+let reduction_prime_2prime_with_carry #c x result  = 
+  let len = getCoordinateLenU64 c in
+  
+  let cin = Lib.Buffer.index x len in
+  let x_ = Lib.Buffer.sub x (size 0) len in
+  let x__ = Lib.Buffer.sub x len len in 
+
+  let h0 = ST.get() in 
+  FStar.Math.Lemmas.pow2_plus 64 (v (getCoordinateLenU64 c) * 64);
+  lseq_upperbound1 (as_seq h0 x) (v (getCoordinateLenU64 c) + 1) (2 * v (getCoordinateLenU64 c) - v (getCoordinateLenU64 c) - 1);
+  lseq_as_nat_definiton (as_seq h0 x) (v (getCoordinateLenU64 c) + 1);
+
+  lemma_lseq_as_seq_extension (as_seq h0 (gsub x (size 0) (getCoordinateLenU64 c))) (as_seq h0 x) (v (getCoordinateLenU64 c));
+  reduction_prime_2prime_with_carry_cin cin x_ result
+
+
+let reduction_prime_2prime_order #c x result  =
+   push_frame();
+  let len = getCoordinateLenU64 c in
+  let tempBuffer = create len (u64 0) in
+    let h0 = ST.get() in
+  let r = sub_bn_order x tempBuffer in
+    let h1 = ST.get() in 
+  lemma_mod_plus (as_nat c h0 x) (-1) (getOrder #c);
+  lseq_upperbound #(v (getCoordinateLenU64 c)) (as_seq h0 x); 
+  cmovznz4 r tempBuffer x result;
+    let h2 = ST.get() in 
+  pop_frame()
