code/ecdsa/Hacl.Impl.ECDSA.LowLevel.fsti
@@ -1,0 +1,26 @@
+module Hacl.Impl.ECDSA.LowLevel
+
+open FStar.HyperStack.All
+open FStar.HyperStack
+module ST = FStar.HyperStack.ST
+
+open Lib.IntTypes
+open Lib.Buffer
+
+open Spec.ECC
+open Spec.ECC.Curves
+open Hacl.Spec.EC.Definition
+
+open FStar.Mul
+
+
+val reduction_prime_2prime_with_carry: #c: curve -> x: widefelem c -> result: felem c ->
+  Stack unit 
+  (requires fun h -> live h x /\ live h result /\  eq_or_disjoint x result /\ wide_as_nat c h x < 2 * getOrder #c)
+  (ensures fun h0 _ h1 -> modifies (loc result) h0 h1 /\ as_nat c h1 result = wide_as_nat c h0 x % getOrder #c)  
+
+val reduction_prime_2prime_order: #c: curve -> x: felem c -> result: felem c -> 
+  Stack unit 
+  (requires fun h -> live h x /\ live h result /\ eq_or_disjoint x result)
+  (ensures fun h0 _ h1 -> modifies (loc result) h0 h1 /\ as_nat c h1 result == as_nat c h0 x % getOrder #c)  
+
